To explore derivative of [[logaritm]]s, we first establish that it is the inverse of the derivative of an [[exponential]]. Moreover, as it happens we have the [[identity_derivative]], which is an [[exponential]].
Therefore, we simply take the [[implicit_derivative]]:
$$
y = \ln x \implies e^y = x
$$
$$
e^y y' = 1 \implies y' = \frac{1}{e^y} \implies y' = \frac{1}{x}
$$
This let's use calculate the derivative of $\ln x$ and using [[logaritm_laws]], we can calculate the derivative of other logarithms by turning it into $\ln x$.