Given two series:
$$
\sum_{i = 0}^{\infty} a_{i} \land \sum_{i = 0}^{\infty} b_{i}
$$
Such that $0 \leq a_{i} \leq b_{i}$ :
Consequently if,
$$
\sum_{i = m}^{\infty} b_{i} < \varepsilon
$$
Then, we have that :
$$
a_{m} \leq b_{m} \land a_{m + 1} \leq b_{m+1} \implies a_{m} + a_{m+1} \leq b_{m} + b_{m+1}
$$
Which means :
$$
\sum_{i = m}^{\infty} a_{i} \leq \sum_{i = m}^{\infty} b_{i} < \varepsilon
$$
Consequently, we have that the convergence of the $b_{i}$ series implies the convergence of $a_{i}$
